driver/ParallelPolOptCorrect.v
@@ -1,0 +1,937 @@
+Require Import ImpureAlarmConfig.
+Require Import Vpl.Impure.
+
+Require Import ISSValidatorCorrect.
+Require Import PolIRs.
+Require Import PolOpt.
+Require Import ParallelPolOpt.
+Require Import Result.
+
+Local Open Scope impure_scope.
+
+Module ParallelPolOptCorrect (PolIRs: POLIRS).
+
+Module Core := ParallelPolOpt PolIRs.
+Module CoreOpt := PolOpt PolIRs.
+Module ISSValidatorCorrectCore := ISSValidatorCorrect PolIRs.
+Module LoopIR := PolIRs.Loop.
+Module PolyLang := PolIRs.PolyLang.
+Module State := PolIRs.State.
+Module ParallelLoop := Core.ParallelCodegenCore.ParallelLoop.
+
+Lemma checked_parallel_current_annotated_codegen_at_correct :
+  forall pol d pl st st',
+    mayReturn (Core.checked_parallel_current_annotated_codegen_at pol d) (Okk pl) ->
+    PolyLang.wf_pprog_general pol ->
+    ParallelLoop.semantics pl st st' ->
+    exists st'',
+      PolyLang.instance_list_semantics pol st st'' /\ State.eq st' st''.
+Proof.
+  intros pol d pl st st' Hopt Hwf Hsem.
+  unfold Core.checked_parallel_current_annotated_codegen_at in Hopt.
+  eapply Core.checked_parallel_current_annotated_codegen_correct; eauto.
+Qed.
+
+Lemma try_verified_tiling_after_phase_mid_poly_correct :
+  forall pol_mid mid_scop after_scop pol_out st st',
+    PolyLang.wf_pprog_affine pol_mid ->
+    mayReturn
+      (Core.try_verified_tiling_after_phase_mid_poly pol_mid mid_scop after_scop)
+      pol_out ->
+    PolyLang.instance_list_semantics pol_out st st' ->
+    exists st'',
+      PolyLang.instance_list_semantics pol_mid st st'' /\ State.eq st' st''.
+Proof.
+  intros pol_mid mid_scop after_scop pol_out st st' Hwf_mid Hopt Hsem_out.
+  unfold Core.try_verified_tiling_after_phase_mid_poly in Hopt.
+  remember (Core.CoreOpt.infer_tiling_witness_scops mid_scop after_scop) as wsres
+    eqn:Hws.
+  destruct wsres as [ws|msg].
+  { remember (Core.ValidatorCore.import_canonical_tiled_after_poly pol_mid after_scop ws)
+      as after_res eqn:Hafter.
+    destruct after_res as [pol_after|msg_after].
+    { simpl in Hopt.
+      bind_imp_destruct Hopt ok Hcheck.
+      destruct ok.
+      { eapply mayReturn_pure in Hopt. subst pol_out.
+        pose proof
+          (Core.ValidatorCore.checked_tiling_validate_poly_implies_wf_after
+             pol_mid pol_after ws Hcheck)
+          as Hwf_after.
+        pose proof
+          (proj1 (PolyLang.instance_list_semantics_current_view_iff
+                    pol_after st st' Hwf_after) Hsem_out)
+          as Hsem_after.
+        destruct
+          (Core.ValidatorCore.checked_tiling_validate_poly_correct
+             pol_mid pol_after ws st st' Hcheck Hsem_after)
+          as [st_mid [Hmid_sem Heq_mid]].
+        exists st_mid.
+        split; assumption. }
+      { eapply mayReturn_pure in Hopt. subst pol_out.
+        exists st'. split; auto. eapply State.eq_refl. } }
+    { simpl in Hopt.
+      eapply mayReturn_pure in Hopt. subst pol_out.
+      exists st'. split; auto. eapply State.eq_refl. } }
+  { simpl in Hopt.
+    eapply mayReturn_pure in Hopt. subst pol_out.
+    exists st'. split; auto. eapply State.eq_refl. }
+Qed.
+
+Lemma try_verified_tiling_after_phase_mid_poly_wf :
+  forall pol_mid mid_scop after_scop pol_out,
+    PolyLang.wf_pprog_affine pol_mid ->
+    mayReturn
+      (Core.try_verified_tiling_after_phase_mid_poly pol_mid mid_scop after_scop)
+      pol_out ->
+    PolyLang.wf_pprog_general pol_out.
+Proof.
+  intros pol_mid mid_scop after_scop pol_out Hwf_mid Hopt.
+  unfold Core.try_verified_tiling_after_phase_mid_poly in Hopt.
+  remember (Core.CoreOpt.infer_tiling_witness_scops mid_scop after_scop) as wsres
+    eqn:Hws.
+  destruct wsres as [ws|msg].
+  { remember (Core.ValidatorCore.import_canonical_tiled_after_poly pol_mid after_scop ws)
+      as after_res eqn:Hafter.
+    destruct after_res as [pol_after|msg_after].
+    { simpl in Hopt.
+      bind_imp_destruct Hopt ok Hcheck.
+      destruct ok.
+      { eapply mayReturn_pure in Hopt. subst pol_out.
+        pose proof
+          (Core.ValidatorCore.checked_tiling_validate_poly_implies_wf_after
+             pol_mid pol_after ws Hcheck)
+          as Hwf_after.
+        pose proof
+          (PolyLang.wf_pprog_general_current_view_affine pol_after Hwf_after)
+          as Hwf_cur_aff.
+        eapply PolyLang.wf_pprog_affine_implies_wf_pprog_general; eauto. }
+      { eapply mayReturn_pure in Hopt. subst pol_out.
+        eapply PolyLang.wf_pprog_affine_implies_wf_pprog_general; eauto. } }
+    { simpl in Hopt.
+      eapply mayReturn_pure in Hopt. subst pol_out.
+      eapply PolyLang.wf_pprog_affine_implies_wf_pprog_general; eauto. } }
+  { simpl in Hopt.
+    eapply mayReturn_pure in Hopt. subst pol_out.
+    eapply PolyLang.wf_pprog_affine_implies_wf_pprog_general; eauto. }
+Qed.
+
+Lemma try_phase_pipeline_from_source_pol_poly_correct :
+  forall pol_source phase_runner before_scop pol_out st st',
+    PolyLang.wf_pprog_affine pol_source ->
+    mayReturn
+      (Core.try_phase_pipeline_from_source_pol_poly
+         pol_source phase_runner before_scop)
+      pol_out ->
+    PolyLang.instance_list_semantics pol_out st st' ->
+    exists st'',
+      PolyLang.instance_list_semantics pol_source st st'' /\ State.eq st' st''.
+Proof.
+  intros pol_source phase_runner before_scop pol_out st st'
+         Hwf_source Hopt Hsem_out.
+  unfold Core.try_phase_pipeline_from_source_pol_poly in Hopt.
+  destruct (phase_runner before_scop) as [[mid_scop after_scop]|msg] eqn:Hphase.
+  - destruct (Core.PolyLang.from_openscop_like_source pol_source mid_scop)
+      as [pol_mid|msg_mid] eqn:Hmid.
+    + bind_imp_destruct Hopt affine_ok Haff.
+      destruct affine_ok.
+      * pose proof
+          (Core.ValidatorCore.validate_preserve_wf_pprog
+             pol_source pol_mid _ Haff eq_refl)
+          as [_ Hwf_mid].
+        pose proof
+          (try_verified_tiling_after_phase_mid_poly_correct
+             pol_mid mid_scop after_scop pol_out st st'
+             Hwf_mid Hopt Hsem_out)
+          as Hmid_corr.
+        destruct Hmid_corr as [st_mid [Hmid_sem Heq_mid]].
+        pose proof
+          (Core.ValidatorCore.validate_correct
+             pol_source pol_mid st st_mid true Haff eq_refl Hmid_sem)
+          as Haff_corr.
+        destruct Haff_corr as [st_src [Hsrc_sem Heq_src]].
+        exists st_src.
+        split; auto.
+        eapply State.eq_trans; eauto.
+      * eapply CoreOpt.scheduler'_correct; eauto.
+    + eapply CoreOpt.scheduler'_correct; eauto.
+  - eapply CoreOpt.scheduler'_correct; eauto.
+Qed.
+
+Lemma try_phase_pipeline_from_source_pol_poly_wf :
+  forall pol_source phase_runner before_scop pol_out,
+    PolyLang.wf_pprog_affine pol_source ->
+    mayReturn
+      (Core.try_phase_pipeline_from_source_pol_poly
+         pol_source phase_runner before_scop)
+      pol_out ->
+    PolyLang.wf_pprog_general pol_out.
+Proof.
+  intros pol_source phase_runner before_scop pol_out Hwf_source Hopt.
+  unfold Core.try_phase_pipeline_from_source_pol_poly in Hopt.
+  destruct (phase_runner before_scop) as [[mid_scop after_scop]|msg] eqn:Hphase.
+  - destruct (Core.PolyLang.from_openscop_like_source pol_source mid_scop)
+      as [pol_mid|msg_mid] eqn:Hmid.
+    + bind_imp_destruct Hopt affine_ok Haff.
+      destruct affine_ok.
+      * pose proof
+          (Core.ValidatorCore.validate_preserve_wf_pprog
+             pol_source pol_mid _ Haff eq_refl)
+          as [_ Hwf_mid].
+        eapply try_verified_tiling_after_phase_mid_poly_wf; eauto.
+      * pose proof
+          (CoreOpt.scheduler'_preserve_wf
+             pol_source pol_out Hwf_source pol_out Hopt eq_refl)
+          as Hwf_out.
+        eapply PolyLang.wf_pprog_affine_implies_wf_pprog_general; eauto.
+    + pose proof
+        (CoreOpt.scheduler'_preserve_wf
+           pol_source pol_out Hwf_source pol_out Hopt eq_refl)
+        as Hwf_out.
+      eapply PolyLang.wf_pprog_affine_implies_wf_pprog_general; eauto.
+  - pose proof
+      (CoreOpt.scheduler'_preserve_wf
+         pol_source pol_out Hwf_source pol_out Hopt eq_refl)
+      as Hwf_out.
+    eapply PolyLang.wf_pprog_affine_implies_wf_pprog_general; eauto.
+Qed.
+
+Lemma phase_pipeline_opt_prepared_from_poly_no_iss_poly_correct :
+  forall pol pol_out st st',
+    PolyLang.wf_pprog_affine pol ->
+    mayReturn (Core.phase_pipeline_opt_prepared_from_poly_no_iss_poly pol) pol_out ->
+    PolyLang.instance_list_semantics pol_out st st' ->
+    exists st'',
+      PolyLang.instance_list_semantics pol st st'' /\ State.eq st' st''.
+Proof.
+  intros pol pol_out st st' Hwf Hopt Hsem_out.
+  unfold Core.phase_pipeline_opt_prepared_from_poly_no_iss_poly in Hopt.
+  destruct (Core.CoreOpt.has_nonscalar_stmt pol) eqn:Hnonscalar.
+  { destruct (Core.CoreOpt.export_for_phase_scheduler pol) as [before_scop|] eqn:Hbefore.
+    { simpl in Hopt.
+      eapply try_phase_pipeline_from_source_pol_poly_correct.
+      - exact Hwf.
+      - exact Hopt.
+      - exact Hsem_out. }
+    { simpl in Hopt.
+      eapply CoreOpt.scheduler'_correct.
+      - exact Hopt.
+      - exact Hsem_out. } }
+  { simpl in Hopt.
+    eapply mayReturn_pure in Hopt. subst pol_out.
+    exists st'. split; auto. eapply State.eq_refl. }
+Qed.
+
+Lemma phase_pipeline_opt_prepared_from_poly_no_iss_poly_wf :
+  forall pol pol_out,
+    PolyLang.wf_pprog_affine pol ->
+    mayReturn (Core.phase_pipeline_opt_prepared_from_poly_no_iss_poly pol) pol_out ->
+    PolyLang.wf_pprog_general pol_out.
+Proof.
+  intros pol pol_out Hwf Hopt.
+  unfold Core.phase_pipeline_opt_prepared_from_poly_no_iss_poly in Hopt.
+  destruct (Core.CoreOpt.has_nonscalar_stmt pol) eqn:Hnonscalar.
+  { destruct (Core.CoreOpt.export_for_phase_scheduler pol) as [before_scop|] eqn:Hbefore.
+    { simpl in Hopt.
+      eapply try_phase_pipeline_from_source_pol_poly_wf.
+      - exact Hwf.
+      - exact Hopt. }
+    { simpl in Hopt.
+      pose proof
+        (CoreOpt.scheduler'_preserve_wf pol pol_out Hwf pol_out Hopt eq_refl)
+        as Hwf_out.
+      eapply PolyLang.wf_pprog_affine_implies_wf_pprog_general; eauto. } }
+  { simpl in Hopt.
+    eapply mayReturn_pure in Hopt. subst pol_out.
+    eapply PolyLang.wf_pprog_affine_implies_wf_pprog_general; eauto. }
+Qed.
+
+Lemma try_checked_iss_phase_pipeline_from_poly_poly_correct :
+  forall pol before_scop pol_out st st',
+    PolyLang.wf_pprog_affine pol ->
+    mayReturn
+      (Core.try_checked_iss_phase_pipeline_from_poly_poly pol before_scop)
+      pol_out ->
+    PolyLang.instance_list_semantics pol_out st st' ->
+    exists st'',
+      PolyLang.instance_list_semantics pol st st'' /\ State.eq st' st''.
+Proof.
+  intros pol before_scop pol_out st st' Hwf Hopt Hsem_out.
+  unfold Core.try_checked_iss_phase_pipeline_from_poly_poly in Hopt.
+  destruct (Core.CoreOpt.infer_iss_from_source_scop pol before_scop) as [iss_opt|msg]
+    eqn:Hiss_infer.
+  - destruct iss_opt as [[pol_iss w]|].
+    + destruct (Core.ValidatorCore.checked_iss_complete_cut_shape_validate pol pol_iss w)
+        eqn:Hiss_check.
+      * bind_imp_destruct Hopt iss_wf Hiss_wf.
+        destruct iss_wf.
+        -- pose proof
+             (CoreOpt.check_wf_polyprog_affine_correct pol_iss _ Hiss_wf eq_refl)
+             as Hwf_iss.
+           pose proof
+             (try_phase_pipeline_from_source_pol_poly_correct
+                pol_iss
+                CoreOpt.run_pluto_phase_pipeline_with_iss
+                before_scop
+                pol_out st st' Hwf_iss Hopt Hsem_out)
+             as Hiss_corr.
+           destruct Hiss_corr as [st_iss [Hiss_sem Heq_iss]].
+           pose proof
+             (ISSValidatorCorrectCore
+                .checked_iss_complete_cut_shape_validate_semantics_correct
+                pol pol_iss w st st_iss Hiss_check Hiss_sem)
+             as Hback.
+           destruct Hback as [st_src [Hsrc_sem Heq_src]].
+           exists st_src.
+           split; auto.
+           eapply State.eq_trans; eauto.
+        -- eapply try_phase_pipeline_from_source_pol_poly_correct; eauto.
+      * eapply try_phase_pipeline_from_source_pol_poly_correct; eauto.
+    + eapply try_phase_pipeline_from_source_pol_poly_correct; eauto.
+  - eapply try_phase_pipeline_from_source_pol_poly_correct; eauto.
+Qed.
+
+Lemma try_checked_iss_phase_pipeline_from_poly_poly_wf :
+  forall pol before_scop pol_out,
+    PolyLang.wf_pprog_affine pol ->
+    mayReturn
+      (Core.try_checked_iss_phase_pipeline_from_poly_poly pol before_scop)
+      pol_out ->
+    PolyLang.wf_pprog_general pol_out.
+Proof.
+  intros pol before_scop pol_out Hwf Hopt.
+  unfold Core.try_checked_iss_phase_pipeline_from_poly_poly in Hopt.
+  destruct (Core.CoreOpt.infer_iss_from_source_scop pol before_scop) as [iss_opt|msg]
+    eqn:Hiss_infer.
+  - destruct iss_opt as [[pol_iss w]|].
+    + destruct (Core.ValidatorCore.checked_iss_complete_cut_shape_validate pol pol_iss w)
+        eqn:Hiss_check.
+      * bind_imp_destruct Hopt iss_wf Hiss_wf.
+        destruct iss_wf.
+        -- pose proof
+             (CoreOpt.check_wf_polyprog_affine_correct pol_iss _ Hiss_wf eq_refl)
+             as Hwf_iss.
+           eapply try_phase_pipeline_from_source_pol_poly_wf; eauto.
+        -- eapply try_phase_pipeline_from_source_pol_poly_wf; eauto.
+      * eapply try_phase_pipeline_from_source_pol_poly_wf; eauto.
+    + eapply try_phase_pipeline_from_source_pol_poly_wf; eauto.
+  - eapply try_phase_pipeline_from_source_pol_poly_wf; eauto.
+Qed.
+
+Lemma phase_pipeline_opt_prepared_from_poly_with_iss_poly_correct :
+  forall pol pol_out st st',
+    PolyLang.wf_pprog_affine pol ->
+    mayReturn (Core.phase_pipeline_opt_prepared_from_poly_with_iss_poly pol) pol_out ->
+    PolyLang.instance_list_semantics pol_out st st' ->
+    exists st'',
+      PolyLang.instance_list_semantics pol st st'' /\ State.eq st' st''.
+Proof.
+  intros pol pol_out st st' Hwf Hopt Hsem_out.
+  unfold Core.phase_pipeline_opt_prepared_from_poly_with_iss_poly in Hopt.
+  destruct (Core.CoreOpt.has_nonscalar_stmt pol) eqn:Hnonscalar.
+  { destruct (Core.CoreOpt.export_for_phase_scheduler pol) as [before_scop|] eqn:Hbefore.
+    { simpl in Hopt.
+      eapply try_checked_iss_phase_pipeline_from_poly_poly_correct.
+      - exact Hwf.
+      - exact Hopt.
+      - exact Hsem_out. }
+    { simpl in Hopt.
+      eapply CoreOpt.scheduler'_correct.
+      - exact Hopt.
+      - exact Hsem_out. } }
+  { simpl in Hopt.
+    eapply mayReturn_pure in Hopt. subst pol_out.
+    exists st'. split; auto. eapply State.eq_refl. }
+Qed.
+
+Lemma phase_pipeline_opt_prepared_from_poly_with_iss_poly_wf :
+  forall pol pol_out,
+    PolyLang.wf_pprog_affine pol ->
+    mayReturn (Core.phase_pipeline_opt_prepared_from_poly_with_iss_poly pol) pol_out ->
+    PolyLang.wf_pprog_general pol_out.
+Proof.
+  intros pol pol_out Hwf Hopt.
+  unfold Core.phase_pipeline_opt_prepared_from_poly_with_iss_poly in Hopt.
+  destruct (Core.CoreOpt.has_nonscalar_stmt pol) eqn:Hnonscalar.
+  { destruct (Core.CoreOpt.export_for_phase_scheduler pol) as [before_scop|] eqn:Hbefore.
+    { simpl in Hopt.
+      eapply try_checked_iss_phase_pipeline_from_poly_poly_wf.
+      - exact Hwf.
+      - exact Hopt. }
+    { simpl in Hopt.
+      pose proof
+        (CoreOpt.scheduler'_preserve_wf pol pol_out Hwf pol_out Hopt eq_refl)
+        as Hwf_out.
+      eapply PolyLang.wf_pprog_affine_implies_wf_pprog_general; eauto. } }
+  { simpl in Hopt.
+    eapply mayReturn_pure in Hopt. subst pol_out.
+    eapply PolyLang.wf_pprog_affine_implies_wf_pprog_general; eauto. }
+Qed.
+
+Lemma iss_only_prepared_from_poly_correct :
+  forall pol pol_out st st',
+    PolyLang.wf_pprog_affine pol ->
+    mayReturn (Core.iss_only_prepared_from_poly pol) pol_out ->
+    PolyLang.instance_list_semantics pol_out st st' ->
+    exists st'',
+      PolyLang.instance_list_semantics pol st st'' /\ State.eq st' st''.
+Proof.
+  intros pol pol_out st st' Hwf Hopt Hsem_out.
+  unfold Core.iss_only_prepared_from_poly in Hopt.
+  destruct (Core.CoreOpt.export_for_phase_scheduler pol) as [before_scop|] eqn:Hbefore.
+  - destruct (Core.CoreOpt.infer_iss_from_source_scop pol before_scop) as [iss_opt|msg]
+      eqn:Hiss_infer.
+    + destruct iss_opt as [[pol_iss w]|].
+      * destruct (Core.ValidatorCore.checked_iss_complete_cut_shape_validate pol pol_iss w)
+          eqn:Hiss_check.
+        -- bind_imp_destruct Hopt iss_wf Hiss_wf.
+           destruct iss_wf.
+           ++ eapply mayReturn_pure in Hopt. subst pol_out.
+              eapply ISSValidatorCorrectCore.checked_iss_complete_cut_shape_validate_semantics_correct;
+                eauto.
+           ++ eapply mayReturn_pure in Hopt. subst pol_out.
+              exists st'. split; auto. eapply State.eq_refl.
+        -- eapply mayReturn_pure in Hopt. subst pol_out.
+           exists st'. split; auto. eapply State.eq_refl.
+      * eapply mayReturn_pure in Hopt. subst pol_out.
+        exists st'. split; auto. eapply State.eq_refl.
+    + eapply mayReturn_pure in Hopt. subst pol_out.
+      exists st'. split; auto. eapply State.eq_refl.
+  - eapply mayReturn_pure in Hopt. subst pol_out.
+    exists st'. split; auto. eapply State.eq_refl.
+Qed.
+
+Lemma iss_only_prepared_from_poly_wf_affine :
+  forall pol pol_out,
+    PolyLang.wf_pprog_affine pol ->
+    mayReturn (Core.iss_only_prepared_from_poly pol) pol_out ->
+    PolyLang.wf_pprog_affine pol_out.
+Proof.
+  intros pol pol_out Hwf Hopt.
+  unfold Core.iss_only_prepared_from_poly in Hopt.
+  destruct (Core.CoreOpt.export_for_phase_scheduler pol) as [before_scop|] eqn:Hbefore.
+  - destruct (Core.CoreOpt.infer_iss_from_source_scop pol before_scop) as [iss_opt|msg]
+      eqn:Hiss_infer.
+    + destruct iss_opt as [[pol_iss w]|].
+      * destruct (Core.ValidatorCore.checked_iss_complete_cut_shape_validate pol pol_iss w)
+          eqn:Hiss_check.
+        -- bind_imp_destruct Hopt iss_wf Hiss_wf.
+           destruct iss_wf.
+           ++ eapply mayReturn_pure in Hopt. subst pol_out.
+              eapply CoreOpt.check_wf_polyprog_affine_correct.
+              ** exact Hiss_wf.
+              ** reflexivity.
+           ++ eapply mayReturn_pure in Hopt. subst pol_out. exact Hwf.
+        -- eapply mayReturn_pure in Hopt. subst pol_out. exact Hwf.
+      * eapply mayReturn_pure in Hopt. subst pol_out. exact Hwf.
+    + eapply mayReturn_pure in Hopt. subst pol_out. exact Hwf.
+  - eapply mayReturn_pure in Hopt. subst pol_out. exact Hwf.
+Qed.
+
+Lemma iss_affine_prepared_from_poly_correct :
+  forall pol pol_out st st',
+    PolyLang.wf_pprog_affine pol ->
+    mayReturn (Core.iss_affine_prepared_from_poly pol) pol_out ->
+    PolyLang.instance_list_semantics pol_out st st' ->
+    exists st'',
+      PolyLang.instance_list_semantics pol st st'' /\ State.eq st' st''.
+Proof.
+  intros pol pol_out st st' Hwf Hopt Hsem_out.
+  unfold Core.iss_affine_prepared_from_poly in Hopt.
+  bind_imp_destruct Hopt pol_iss Hiss.
+  pose proof
+    (iss_only_prepared_from_poly_wf_affine pol pol_iss Hwf Hiss)
+    as Hwf_iss.
+  pose proof
+    (CoreOpt.scheduler'_correct pol_iss st st' pol_out Hopt Hsem_out)
+    as Haff_corr.
+  destruct Haff_corr as [st_iss [Hiss_sem Heq_iss]].
+  pose proof
+    (iss_only_prepared_from_poly_correct pol pol_iss st st_iss Hwf Hiss Hiss_sem)
+    as Hsrc_corr.
+  destruct Hsrc_corr as [st_src [Hsrc_sem Heq_src]].
+  exists st_src.
+  split; auto.
+  eapply State.eq_trans; eauto.
+Qed.
+
+Lemma iss_affine_prepared_from_poly_wf_affine :
+  forall pol pol_out,
+    PolyLang.wf_pprog_affine pol ->
+    mayReturn (Core.iss_affine_prepared_from_poly pol) pol_out ->
+    PolyLang.wf_pprog_affine pol_out.
+Proof.
+  intros pol pol_out Hwf Hopt.
+  unfold Core.iss_affine_prepared_from_poly in Hopt.
+  bind_imp_destruct Hopt pol_iss Hiss.
+  pose proof
+    (iss_only_prepared_from_poly_wf_affine pol pol_iss Hwf Hiss)
+    as Hwf_iss.
+  eapply CoreOpt.scheduler'_preserve_wf; eauto.
+Qed.
+
+Lemma parallel_current_identity_prepared_from_poly_correct :
+  forall pol d pl st st',
+    PolyLang.wf_pprog_affine pol ->
+    mayReturn (Core.parallel_current_identity_prepared_from_poly pol d) (Okk pl) ->
+    ParallelLoop.semantics pl st st' ->
+    exists st'',
+      PolyLang.instance_list_semantics pol st st'' /\ State.eq st' st''.
+Proof.
+  intros pol d pl st st' Hwf Hopt Hsem.
+  unfold Core.parallel_current_identity_prepared_from_poly in Hopt.
+  eapply checked_parallel_current_annotated_codegen_at_correct; eauto.
+  eapply PolyLang.wf_pprog_affine_implies_wf_pprog_general; eauto.
+Qed.
+
+Lemma parallel_current_affine_prepared_from_poly_correct :
+  forall pol d pl st st',
+    PolyLang.wf_pprog_affine pol ->
+    mayReturn (Core.parallel_current_affine_prepared_from_poly pol d) (Okk pl) ->
+    ParallelLoop.semantics pl st st' ->
+    exists st'',
+      PolyLang.instance_list_semantics pol st st'' /\ State.eq st' st''.
+Proof.
+  intros pol d pl st st' Hwf Hopt Hsem.
+  unfold Core.parallel_current_affine_prepared_from_poly in Hopt.
+  bind_imp_destruct Hopt pol_mid Hsched.
+  pose proof
+    (CoreOpt.scheduler'_preserve_wf pol pol_mid Hwf pol_mid Hsched eq_refl)
+    as Hwf_mid.
+  pose proof
+    (checked_parallel_current_annotated_codegen_at_correct
+       pol_mid d pl st st' Hopt
+       (PolyLang.wf_pprog_affine_implies_wf_pprog_general _ Hwf_mid)
+       Hsem)
+    as Hmid_corr.
+  destruct Hmid_corr as [st_mid [Hmid_sem Heq_mid]].
+  pose proof
+    (CoreOpt.scheduler'_correct pol st st_mid pol_mid Hsched Hmid_sem)
+    as Hsched_corr.
+  destruct Hsched_corr as [st_src [Hsrc_sem Heq_src]].
+  exists st_src.
+  split; auto.
+  eapply State.eq_trans; eauto.
+Qed.
+
+Lemma parallel_current_prepared_from_poly_correct :
+  forall pol d pl st st',
+    PolyLang.wf_pprog_affine pol ->
+    mayReturn (Core.parallel_current_prepared_from_poly pol d) (Okk pl) ->
+    ParallelLoop.semantics pl st st' ->
+    exists st'',
+      PolyLang.instance_list_semantics pol st st'' /\ State.eq st' st''.
+Proof.
+  intros pol d pl st st' Hwf Hopt Hsem.
+  unfold Core.parallel_current_prepared_from_poly in Hopt.
+  bind_imp_destruct Hopt pol_after Hphase.
+  pose proof
+    (phase_pipeline_opt_prepared_from_poly_no_iss_poly_wf
+       pol pol_after Hwf Hphase)
+    as Hwf_after.
+  pose proof
+    (checked_parallel_current_annotated_codegen_at_correct
+       pol_after d pl st st' Hopt Hwf_after Hsem)
+    as Hafter_corr.
+  destruct Hafter_corr as [st_after [Hafter_sem Heq_after]].
+  pose proof
+    (phase_pipeline_opt_prepared_from_poly_no_iss_poly_correct
+       pol pol_after st st_after Hwf Hphase Hafter_sem)
+    as Hphase_corr.
+  destruct Hphase_corr as [st_src [Hsrc_sem Heq_src]].
+  exists st_src.
+  split; auto.
+  eapply State.eq_trans; eauto.
+Qed.
+
+Lemma parallel_current_identity_prepared_from_poly_with_iss_correct :
+  forall pol d pl st st',
+    PolyLang.wf_pprog_affine pol ->
+    mayReturn (Core.parallel_current_identity_prepared_from_poly_with_iss pol d) (Okk pl) ->
+    ParallelLoop.semantics pl st st' ->
+    exists st'',
+      PolyLang.instance_list_semantics pol st st'' /\ State.eq st' st''.
+Proof.
+  intros pol d pl st st' Hwf Hopt Hsem.
+  unfold Core.parallel_current_identity_prepared_from_poly_with_iss in Hopt.
+  bind_imp_destruct Hopt pol_iss Hiss.
+  pose proof
+    (iss_only_prepared_from_poly_wf_affine pol pol_iss Hwf Hiss)
+    as Hwf_iss.
+  pose proof
+    (checked_parallel_current_annotated_codegen_at_correct
+       pol_iss d pl st st' Hopt
+       (PolyLang.wf_pprog_affine_implies_wf_pprog_general _ Hwf_iss)
+       Hsem)
+    as Hiss_corr.
+  destruct Hiss_corr as [st_iss [Hiss_sem Heq_iss]].
+  pose proof
+    (iss_only_prepared_from_poly_correct pol pol_iss st st_iss Hwf Hiss Hiss_sem)
+    as Hsrc_corr.
+  destruct Hsrc_corr as [st_src [Hsrc_sem Heq_src]].
+  exists st_src.
+  split; auto.
+  eapply State.eq_trans; eauto.
+Qed.
+
+Lemma parallel_current_affine_prepared_from_poly_with_iss_correct :
+  forall pol d pl st st',
+    PolyLang.wf_pprog_affine pol ->
+    mayReturn (Core.parallel_current_affine_prepared_from_poly_with_iss pol d) (Okk pl) ->
+    ParallelLoop.semantics pl st st' ->
+    exists st'',
+      PolyLang.instance_list_semantics pol st st'' /\ State.eq st' st''.
+Proof.
+  intros pol d pl st st' Hwf Hopt Hsem.
+  unfold Core.parallel_current_affine_prepared_from_poly_with_iss in Hopt.
+  bind_imp_destruct Hopt pol_mid Hiss_affine.
+  pose proof
+    (iss_affine_prepared_from_poly_wf_affine pol pol_mid Hwf Hiss_affine)
+    as Hwf_mid.
+  pose proof
+    (checked_parallel_current_annotated_codegen_at_correct
+       pol_mid d pl st st' Hopt
+       (PolyLang.wf_pprog_affine_implies_wf_pprog_general _ Hwf_mid)
+       Hsem)
+    as Hmid_corr.
+  destruct Hmid_corr as [st_mid [Hmid_sem Heq_mid]].
+  pose proof
+    (iss_affine_prepared_from_poly_correct pol pol_mid st st_mid Hwf Hiss_affine Hmid_sem)
+    as Hsrc_corr.
+  destruct Hsrc_corr as [st_src [Hsrc_sem Heq_src]].
+  exists st_src.
+  split; auto.
+  eapply State.eq_trans; eauto.
+Qed.
+
+Lemma parallel_current_prepared_from_poly_with_iss_correct :
+  forall pol d pl st st',
+    PolyLang.wf_pprog_affine pol ->
+    mayReturn (Core.parallel_current_prepared_from_poly_with_iss pol d) (Okk pl) ->
+    ParallelLoop.semantics pl st st' ->
+    exists st'',
+      PolyLang.instance_list_semantics pol st st'' /\ State.eq st' st''.
+Proof.
+  intros pol d pl st st' Hwf Hopt Hsem.
+  unfold Core.parallel_current_prepared_from_poly_with_iss in Hopt.
+  bind_imp_destruct Hopt pol_after Hphase.
+  pose proof
+    (phase_pipeline_opt_prepared_from_poly_with_iss_poly_wf
+       pol pol_after Hwf Hphase)
+    as Hwf_after.
+  pose proof
+    (checked_parallel_current_annotated_codegen_at_correct
+       pol_after d pl st st' Hopt Hwf_after Hsem)
+    as Hafter_corr.
+  destruct Hafter_corr as [st_after [Hafter_sem Heq_after]].
+  pose proof
+    (phase_pipeline_opt_prepared_from_poly_with_iss_poly_correct
+       pol pol_after st st_after Hwf Hphase Hafter_sem)
+    as Hphase_corr.
+  destruct Hphase_corr as [st_src [Hsrc_sem Heq_src]].
+  exists st_src.
+  split; auto.
+  eapply State.eq_trans; eauto.
+Qed.
+
+Theorem Opt_parallel_current_identity_result_correct :
+  forall loop d pl st st',
+    mayReturn (Core.Opt_parallel_current_identity_result loop d) (Okk pl) ->
+    ParallelLoop.semantics pl st st' ->
+    exists st'',
+      LoopIR.semantics loop st st'' /\ State.eq st' st''.
+Proof.
+  intros loop d pl st st' Hopt Hsem.
+  unfold Core.Opt_parallel_current_identity_result in Hopt.
+  bind_imp_destruct Hopt pol0 Hextimp.
+  set (pol := CoreOpt.Strengthen.strengthen_pprog pol0) in *.
+  pose proof Hextimp as Hextok.
+  apply res_to_alarm_correct in Hextok.
+  pose proof
+    (CoreOpt.Strengthen.strengthen_pprog_wf_affine
+       pol0
+       (CoreOpt.extractor_success_wf_pprog_affine loop pol0 Hextok))
+    as Hwf_pol.
+  pose proof
+    (parallel_current_identity_prepared_from_poly_correct
+       pol d pl st st' Hwf_pol Hopt Hsem)
+    as Hphase_corr.
+  destruct Hphase_corr as [st_str [Hstr_sem Heq_str]].
+  eapply CoreOpt.Strengthen.instance_list_semantics_unstrengthen in Hstr_sem.
+  pose proof (CoreOpt.Extractor.extractor_correct loop pol0 st st_str Hextok Hstr_sem)
+    as Hext_corr.
+  destruct Hext_corr as [st_src [Hloop_src Heq_src]].
+  exists st_src.
+  split; auto.
+  eapply State.eq_trans.
+  - exact Heq_str.
+  - exact Heq_src.
+Qed.
+
+Theorem Opt_parallel_current_affine_result_correct :
+  forall loop d pl st st',
+    mayReturn (Core.Opt_parallel_current_affine_result loop d) (Okk pl) ->
+    ParallelLoop.semantics pl st st' ->
+    exists st'',
+      LoopIR.semantics loop st st'' /\ State.eq st' st''.
+Proof.
+  intros loop d pl st st' Hopt Hsem.
+  unfold Core.Opt_parallel_current_affine_result in Hopt.
+  bind_imp_destruct Hopt pol0 Hextimp.
+  set (pol := CoreOpt.Strengthen.strengthen_pprog pol0) in *.
+  pose proof Hextimp as Hextok.
+  apply res_to_alarm_correct in Hextok.
+  pose proof
+    (CoreOpt.Strengthen.strengthen_pprog_wf_affine
+       pol0
+       (CoreOpt.extractor_success_wf_pprog_affine loop pol0 Hextok))
+    as Hwf_pol.
+  pose proof
+    (parallel_current_affine_prepared_from_poly_correct
+       pol d pl st st' Hwf_pol Hopt Hsem)
+    as Hphase_corr.
+  destruct Hphase_corr as [st_str [Hstr_sem Heq_str]].
+  eapply CoreOpt.Strengthen.instance_list_semantics_unstrengthen in Hstr_sem.
+  pose proof (CoreOpt.Extractor.extractor_correct loop pol0 st st_str Hextok Hstr_sem)
+    as Hext_corr.
+  destruct Hext_corr as [st_src [Hloop_src Heq_src]].
+  exists st_src.
+  split; auto.
+  eapply State.eq_trans.
+  - exact Heq_str.
+  - exact Heq_src.
+Qed.
+
+Theorem Opt_parallel_current_result_correct :
+  forall loop d pl st st',
+    mayReturn (Core.Opt_parallel_current_result loop d) (Okk pl) ->
+    ParallelLoop.semantics pl st st' ->
+    exists st'',
+      LoopIR.semantics loop st st'' /\ State.eq st' st''.
+Proof.
+  intros loop d pl st st' Hopt Hsem.
+  unfold Core.Opt_parallel_current_result in Hopt.
+  bind_imp_destruct Hopt pol0 Hextimp.
+  set (pol := CoreOpt.Strengthen.strengthen_pprog pol0) in *.
+  pose proof Hextimp as Hextok.
+  apply res_to_alarm_correct in Hextok.
+  pose proof
+    (CoreOpt.Strengthen.strengthen_pprog_wf_affine
+       pol0
+       (CoreOpt.extractor_success_wf_pprog_affine loop pol0 Hextok))
+    as Hwf_pol.
+  pose proof
+    (parallel_current_prepared_from_poly_correct
+       pol d pl st st' Hwf_pol Hopt Hsem)
+    as Hphase_corr.
+  destruct Hphase_corr as [st_str [Hstr_sem Heq_str]].
+  eapply CoreOpt.Strengthen.instance_list_semantics_unstrengthen in Hstr_sem.
+  pose proof (CoreOpt.Extractor.extractor_correct loop pol0 st st_str Hextok Hstr_sem)
+    as Hext_corr.
+  destruct Hext_corr as [st_src [Hloop_src Heq_src]].
+  exists st_src.
+  split; auto.
+  eapply State.eq_trans.
+  - exact Heq_str.
+  - exact Heq_src.
+Qed.
+
+Theorem Opt_parallel_current_identity_with_iss_result_correct :
+  forall loop d pl st st',
+    mayReturn (Core.Opt_parallel_current_identity_with_iss_result loop d) (Okk pl) ->
+    ParallelLoop.semantics pl st st' ->
+    exists st'',
+      LoopIR.semantics loop st st'' /\ State.eq st' st''.
+Proof.
+  intros loop d pl st st' Hopt Hsem.
+  unfold Core.Opt_parallel_current_identity_with_iss_result in Hopt.
+  bind_imp_destruct Hopt pol0 Hextimp.
+  set (pol := CoreOpt.Strengthen.strengthen_pprog pol0) in *.
+  pose proof Hextimp as Hextok.
+  apply res_to_alarm_correct in Hextok.
+  pose proof
+    (CoreOpt.Strengthen.strengthen_pprog_wf_affine
+       pol0
+       (CoreOpt.extractor_success_wf_pprog_affine loop pol0 Hextok))
+    as Hwf_pol.
+  pose proof
+    (parallel_current_identity_prepared_from_poly_with_iss_correct
+       pol d pl st st' Hwf_pol Hopt Hsem)
+    as Hphase_corr.
+  destruct Hphase_corr as [st_str [Hstr_sem Heq_str]].
+  eapply CoreOpt.Strengthen.instance_list_semantics_unstrengthen in Hstr_sem.
+  pose proof (CoreOpt.Extractor.extractor_correct loop pol0 st st_str Hextok Hstr_sem)
+    as Hext_corr.
+  destruct Hext_corr as [st_src [Hloop_src Heq_src]].
+  exists st_src.
+  split; auto.
+  eapply State.eq_trans.
+  - exact Heq_str.
+  - exact Heq_src.
+Qed.
+
+Theorem Opt_parallel_current_affine_with_iss_result_correct :
+  forall loop d pl st st',
+    mayReturn (Core.Opt_parallel_current_affine_with_iss_result loop d) (Okk pl) ->
+    ParallelLoop.semantics pl st st' ->
+    exists st'',
+      LoopIR.semantics loop st st'' /\ State.eq st' st''.
+Proof.
+  intros loop d pl st st' Hopt Hsem.
+  unfold Core.Opt_parallel_current_affine_with_iss_result in Hopt.
+  bind_imp_destruct Hopt pol0 Hextimp.
+  set (pol := CoreOpt.Strengthen.strengthen_pprog pol0) in *.
+  pose proof Hextimp as Hextok.
+  apply res_to_alarm_correct in Hextok.
+  pose proof
+    (CoreOpt.Strengthen.strengthen_pprog_wf_affine
+       pol0
+       (CoreOpt.extractor_success_wf_pprog_affine loop pol0 Hextok))
+    as Hwf_pol.
+  pose proof
+    (parallel_current_affine_prepared_from_poly_with_iss_correct
+       pol d pl st st' Hwf_pol Hopt Hsem)
+    as Hphase_corr.
+  destruct Hphase_corr as [st_str [Hstr_sem Heq_str]].
+  eapply CoreOpt.Strengthen.instance_list_semantics_unstrengthen in Hstr_sem.
+  pose proof (CoreOpt.Extractor.extractor_correct loop pol0 st st_str Hextok Hstr_sem)
+    as Hext_corr.
+  destruct Hext_corr as [st_src [Hloop_src Heq_src]].
+  exists st_src.
+  split; auto.
+  eapply State.eq_trans.
+  - exact Heq_str.
+  - exact Heq_src.
+Qed.
+
+Theorem Opt_parallel_current_with_iss_result_correct :
+  forall loop d pl st st',
+    mayReturn (Core.Opt_parallel_current_with_iss_result loop d) (Okk pl) ->
+    ParallelLoop.semantics pl st st' ->
+    exists st'',
+      LoopIR.semantics loop st st'' /\ State.eq st' st''.
+Proof.
+  intros loop d pl st st' Hopt Hsem.
+  unfold Core.Opt_parallel_current_with_iss_result in Hopt.
+  bind_imp_destruct Hopt pol0 Hextimp.
+  set (pol := CoreOpt.Strengthen.strengthen_pprog pol0) in *.
+  pose proof Hextimp as Hextok.
+  apply res_to_alarm_correct in Hextok.
+  pose proof
+    (CoreOpt.Strengthen.strengthen_pprog_wf_affine
+       pol0
+       (CoreOpt.extractor_success_wf_pprog_affine loop pol0 Hextok))
+    as Hwf_pol.
+  pose proof
+    (parallel_current_prepared_from_poly_with_iss_correct
+       pol d pl st st' Hwf_pol Hopt Hsem)
+    as Hphase_corr.
+  destruct Hphase_corr as [st_str [Hstr_sem Heq_str]].
+  eapply CoreOpt.Strengthen.instance_list_semantics_unstrengthen in Hstr_sem.
+  pose proof (CoreOpt.Extractor.extractor_correct loop pol0 st st_str Hextok Hstr_sem)
+    as Hext_corr.
+  destruct Hext_corr as [st_src [Hloop_src Heq_src]].
+  exists st_src.
+  split; auto.
+  eapply State.eq_trans.
+  - exact Heq_str.
+  - exact Heq_src.
+Qed.
+
+Theorem Opt_parallel_current_identity_correct :
+  forall loop d pl st st',
+    mayReturn (Core.Opt_parallel_current_identity loop d) pl ->
+    ParallelLoop.semantics pl st st' ->
+    exists st'',
+      LoopIR.semantics loop st st'' /\ State.eq st' st''.
+Proof.
+  intros loop d pl st st' Hopt Hsem.
+  unfold Core.Opt_parallel_current_identity in Hopt.
+  bind_imp_destruct Hopt res Hres.
+  pose proof Hopt as Hopt_ok.
+  apply res_to_alarm_correct in Hopt_ok.
+  subst res.
+  eapply Opt_parallel_current_identity_result_correct; eauto.
+Qed.
+
+Theorem Opt_parallel_current_affine_correct :
+  forall loop d pl st st',
+    mayReturn (Core.Opt_parallel_current_affine loop d) pl ->
+    ParallelLoop.semantics pl st st' ->
+    exists st'',
+      LoopIR.semantics loop st st'' /\ State.eq st' st''.
+Proof.
+  intros loop d pl st st' Hopt Hsem.
+  unfold Core.Opt_parallel_current_affine in Hopt.
+  bind_imp_destruct Hopt res Hres.
+  pose proof Hopt as Hopt_ok.
+  apply res_to_alarm_correct in Hopt_ok.
+  subst res.
+  eapply Opt_parallel_current_affine_result_correct; eauto.
+Qed.
+
+Theorem Opt_parallel_current_correct :
+  forall loop d pl st st',
+    mayReturn (Core.Opt_parallel_current loop d) pl ->
+    ParallelLoop.semantics pl st st' ->
+    exists st'',
+      LoopIR.semantics loop st st'' /\ State.eq st' st''.
+Proof.
+  intros loop d pl st st' Hopt Hsem.
+  unfold Core.Opt_parallel_current in Hopt.
+  bind_imp_destruct Hopt res Hres.
+  pose proof Hopt as Hopt_ok.
+  apply res_to_alarm_correct in Hopt_ok.
+  subst res.
+  eapply Opt_parallel_current_result_correct; eauto.
+Qed.
+
+Theorem Opt_parallel_current_identity_with_iss_correct :
+  forall loop d pl st st',
+    mayReturn (Core.Opt_parallel_current_identity_with_iss loop d) pl ->
+    ParallelLoop.semantics pl st st' ->
+    exists st'',
+      LoopIR.semantics loop st st'' /\ State.eq st' st''.
+Proof.
+  intros loop d pl st st' Hopt Hsem.
+  unfold Core.Opt_parallel_current_identity_with_iss in Hopt.
+  bind_imp_destruct Hopt res Hres.
+  pose proof Hopt as Hopt_ok.
+  apply res_to_alarm_correct in Hopt_ok.
+  subst res.
+  eapply Opt_parallel_current_identity_with_iss_result_correct; eauto.
+Qed.
+
+Theorem Opt_parallel_current_affine_with_iss_correct :
+  forall loop d pl st st',
+    mayReturn (Core.Opt_parallel_current_affine_with_iss loop d) pl ->
+    ParallelLoop.semantics pl st st' ->
+    exists st'',
+      LoopIR.semantics loop st st'' /\ State.eq st' st''.
+Proof.
+  intros loop d pl st st' Hopt Hsem.
+  unfold Core.Opt_parallel_current_affine_with_iss in Hopt.
+  bind_imp_destruct Hopt res Hres.
+  pose proof Hopt as Hopt_ok.
+  apply res_to_alarm_correct in Hopt_ok.
+  subst res.
+  eapply Opt_parallel_current_affine_with_iss_result_correct; eauto.
+Qed.
+
+Theorem Opt_parallel_current_with_iss_correct :
+  forall loop d pl st st',
+    mayReturn (Core.Opt_parallel_current_with_iss loop d) pl ->
+    ParallelLoop.semantics pl st st' ->
+    exists st'',
+      LoopIR.semantics loop st st'' /\ State.eq st' st''.
+Proof.
+  intros loop d pl st st' Hopt Hsem.
+  unfold Core.Opt_parallel_current_with_iss in Hopt.
+  bind_imp_destruct Hopt res Hres.
+  pose proof Hopt as Hopt_ok.
+  apply res_to_alarm_correct in Hopt_ok.
+  subst res.
+  eapply Opt_parallel_current_with_iss_result_correct; eauto.
+Qed.
+
+End ParallelPolOptCorrect.
