extraction/extraction.v
@@ -206,6 +206,7 @@ Require Import Ctyping.
 Require Import CPolOpt.
 Require Import TPolOpt.
 Require Import SPolOpt.
+Require Import SParallelPolOpt.
 Require Import STilingOpt.
 Require Import TPolValidator.
 
@@ -213,4 +214,4 @@ Require Import TPolValidator.
 Set Warnings "-extraction-ambiguous-name". (* This warning does not matter *)
 Set Warnings "-extraction-opaque-accessed". (* To be fixed in VPL *)
 
-Separate Extraction Archi Result AST Csyntax BinNums BinPos BinNat Floats Coq.ZArith.BinInt.Z ZArith_dec Ring_polynom_AddOnQ CstrLCF ProgVar LinTerm sample_scop OpenScop OpenScopAST PolyLang CPolIRs CSample1.sample_cpol CSample2.sample_cpol CSample3.sample_cpol Integers Memdata Ctypes Ctyping Initializers Debugging Qcanon NumC CoqAddOn ParallelLoop ParallelCodegen CPolOpt TPolIRs TPolOpt SPolIRs SPolOpt STilingOpt TPolValidator.
+Separate Extraction Archi Result AST Csyntax BinNums BinPos BinNat Floats Coq.ZArith.BinInt.Z ZArith_dec Ring_polynom_AddOnQ CstrLCF ProgVar LinTerm sample_scop OpenScop OpenScopAST PolyLang CPolIRs CSample1.sample_cpol CSample2.sample_cpol CSample3.sample_cpol Integers Memdata Ctypes Ctyping Initializers Debugging Qcanon NumC CoqAddOn ParallelLoop ParallelCodegen CPolOpt TPolIRs TPolOpt SPolIRs SPolOpt SParallelPolOpt STilingOpt TPolValidator.
